lunarlander_sl/ext2/BigStepParallel.thy
@@ -1,728 +1,6 @@
-theory BigStepSimple
-  imports "../Analysis_More"
+theory BigStepParallel
+  imports BigStepSequential
 begin
-
-
-subsection \<open>Extended state\<close>
-
-text \<open>The state of each process consists of the real part, which
-  is a mapping from variable names to real numbers, and an extra
-  part, which can be of arbitrary type 'a.
-\<close>
-datatype 'a estate = EState (rp: state) (ep: 'a)
-
-text \<open>Expressions on an extended state\<close>
-type_synonym 'a eexp = "'a estate \<Rightarrow> real"
-
-text \<open>Predicates on an extended state\<close>
-type_synonym 'a eform = "'a estate \<Rightarrow> bool"
-
-text \<open>Updating some variable in the real part of the state\<close>
-fun upd :: "'a estate \<Rightarrow> var \<Rightarrow> real \<Rightarrow> 'a estate" where
-  "upd (EState r e) x v = EState (r(x := v)) e"
-
-text \<open>Updating entirety of the real part of the state\<close>
-fun updr :: "'a estate \<Rightarrow> state \<Rightarrow> 'a estate" where
-  "updr (EState r e) r2 = EState r2 e"
-
-text \<open>Updating the extra part of the state\<close>
-fun upde :: "'a estate \<Rightarrow> 'a \<Rightarrow> 'a estate" where
-  "upde (EState r e) e2 = EState r e2"
-
-text \<open>Obtain the value of some variable in the real part of the state\<close>
-fun val :: "'a estate \<Rightarrow> var \<Rightarrow> real" where
-  "val (EState r e) v = r v"
-
-text \<open>Taking the real part of the state\<close>
-fun rpart :: "'a estate \<Rightarrow> state" where
-  "rpart (EState r e) = r"
-
-text \<open>Taking the extra part of the state\<close>
-fun epart :: "'a estate \<Rightarrow> 'a" where
-  "epart (EState r e) = e"
-
-text \<open>The following rules allow to simplify expressions
-  involving evaluation and updating the extended state.
-\<close>
-lemma val_upd_simp [simp]:
-  "val (upd s var v) var = v"
-  apply (cases s) by auto
-
-lemma val_upd_simp2 [simp]:
-  "var \<noteq> var2 \<Longrightarrow> val (upd s var v) var2 = val s var2"
-  apply (cases s) by auto
-
-lemma val_upde_simp [simp]:
-  "val (upde s e) var = val s var"
-  apply (cases s) by auto
-
-lemma epart_upd_simp [simp]:
-  "epart (upd s var v) = epart s"
-  apply (cases s) by auto
-
-lemma epart_upde_simp [simp]:
-  "epart (upde s e) = e"
-  apply (cases s) by auto
-
-lemma updr_rpart_simp [simp]:
-  "updr s (rpart s) = s"
-  apply (cases s) by auto
-
-lemma upd_val_simp [simp]:
-  "upd s X (val s X) = s"
-  apply (cases s) by auto
-
-text \<open>The following lemmas need to be invoked by hand\<close>
-lemma updr_rpart_simp1:
-  "updr s ((rpart s)(X := v)) = upd s X v"
-  apply (cases s) by auto
-
-lemma updr_rpart_simp2:
-  "updr s ((rpart s)(X := v, Y := w)) = upd (upd s X v) Y w"
-  apply (cases s) by auto
-
-declare upd.simps [simp del]
-declare updr.simps [simp del]
-declare rpart.simps [simp del]
-declare epart.simps [simp del]
-declare val.simps [simp del]
-
-subsection \<open>Syntax of HCSP\<close>
-
-text \<open>Channel names\<close>
-type_synonym cname = string
-
-text \<open>Process names\<close>
-type_synonym pname = string
-
-text \<open>Readiness information.
-  First component is set of channels that are ready to output.
-  Second component is set of channels that are ready to input.
-\<close>
-type_synonym rdy_info = "cname set \<times> cname set"
-
-text \<open>Communications\<close>
-datatype 'a comm =
-  Send cname "'a eexp"        ("_[!]_" [110,108] 100)
-| Receive cname var           ("_[?]_" [110,108] 100)
-
-text \<open>HCSP processes\<close>
-datatype 'a proc =
-  Cm "'a comm"
-| Skip
-| Assign var "'a eexp"                 ("_ ::= _" [99,95] 94)
-| Basic "'a estate \<Rightarrow> 'a"
-| Error
-| Seq "'a proc" "'a proc"              ("_; _" [91,90] 90)
-| Cond "'a eform" "'a proc" "'a proc"  ("IF _ THEN _ ELSE _ FI" [95,94] 93)
-| Wait "'a eexp"  \<comment> \<open>Waiting for a specified amount of time\<close>
-| IChoice "'a proc" "'a proc"  \<comment> \<open>Nondeterminism\<close>
-| EChoice "('a comm \<times> 'a proc) list"  \<comment> \<open>External choice\<close>
-| Rep "'a proc"   \<comment> \<open>Nondeterministic repetition\<close>
-| Cont ODE "'a eform"  \<comment> \<open>ODE with boundary\<close>
-| Interrupt ODE "'a eform" "('a comm \<times> 'a proc) list" "'a proc" \<comment> \<open>Interrupt\<close>
-
-text \<open>Parallel of several HCSP processes\<close>
-datatype 'a pproc =
-  Single pname "'a proc"
-| Parallel "'a pproc" "cname set" "'a pproc"
-
-text \<open>Set of process names of a parallel process\<close>
-fun proc_of_pproc :: "'a pproc \<Rightarrow> pname set" where
-  "proc_of_pproc (Single pn c) = {pn}"
-| "proc_of_pproc (Parallel p1 chs p2) = proc_of_pproc p1 \<union> proc_of_pproc p2"
-
-text \<open>Global state.
-
-  The global state of a parallel process is represented as a
-  partial mapping from process name to extended state.
-\<close>
-type_synonym 'a gstate = "pname \<Rightarrow> 'a estate option"
-
-text \<open>Global state for a single process\<close>
-definition State :: "pname \<Rightarrow> 'a estate \<Rightarrow> 'a gstate" where
-  "State p s = (\<lambda>p'. if p' = p then Some s else None)"
-
-lemma State_eval [simp]:
-  "State p s p = Some s"
-  by (auto simp add: State_def)
-
-subsection \<open>Traces of sequential programs\<close>
-
-datatype comm_type = In | Out
-
-text \<open>Each trace block is either:
-
-  - Communication block, specified by communication type (In or Out),
-    name of the channel, and the communicated value.
-
-  - Wait block, specified by length of the wait, state as a function
-    of time during the wait, and set of ready communications.
-\<close>
-datatype 'a trace_block =
-  CommBlock comm_type cname real
-| WaitBlock real "real \<Rightarrow> 'a estate" rdy_info
-
-abbreviation "InBlock ch v \<equiv> CommBlock In ch v"
-abbreviation "OutBlock ch v \<equiv> CommBlock Out ch v"
-
-definition WaitBlk :: "real \<Rightarrow> (real \<Rightarrow> 'a estate) \<Rightarrow> rdy_info \<Rightarrow> 'a trace_block" where
-  "WaitBlk d p rdy = WaitBlock d (\<lambda>\<tau>\<in>{0..d}. p \<tau>) rdy"
-
-lemma WaitBlk_eqE:
-  "WaitBlk d p rdy = WaitBlk d2 p2 rdy2 \<Longrightarrow>
-   (d = d2 \<Longrightarrow> rdy = rdy2 \<Longrightarrow> (\<And>t. t \<in> {0..d} \<Longrightarrow> p t = p2 t) \<Longrightarrow> P) \<Longrightarrow> P"
-  unfolding WaitBlk_def restrict_def apply auto by meson
-
-lemma WaitBlk_eqI:
-  "d = d2 \<Longrightarrow> rdy = rdy2 \<Longrightarrow> (\<And>t. t \<in> {0..d} \<Longrightarrow> p t = p2 t) \<Longrightarrow> WaitBlk d p rdy = WaitBlk d2 p2 rdy2"
-  unfolding WaitBlk_def by auto
-
-text \<open>Trace is defined as an ordered list of trace blocks.\<close>
-type_synonym 'a trace = "'a trace_block list"
-
-
-subsection \<open>Big-step semantics\<close>
-
-text \<open>Compute list of ready communications for an external choice\<close>
-
-fun rdy_info_of_list :: "('a \<Rightarrow> rdy_info) \<Rightarrow> 'a list \<Rightarrow> rdy_info" where
-  "rdy_info_of_list f [] = ({}, {})"
-| "rdy_info_of_list f (x # xs) = (
-    let rdy = rdy_info_of_list f xs in
-      (fst (f x) \<union> fst rdy, snd (f x) \<union> snd rdy))"
-
-definition rdy_of_echoice :: "('a comm \<times> 'a proc) list \<Rightarrow> rdy_info" where
-  "rdy_of_echoice = rdy_info_of_list (\<lambda>es.
-    case es of (ch[!]e, _) \<Rightarrow> ({ch}, {})
-             | (ch[?]var, _) \<Rightarrow> ({}, {ch}))"
-
-text \<open>big_step p s1 tr s2 means executing p starting from
-  state s1 results in a trace tr and final state s2.
-\<close>
-inductive big_step :: "'a proc \<Rightarrow> 'a estate \<Rightarrow> 'a trace \<Rightarrow> 'a estate \<Rightarrow> bool" where
-  skipB: "big_step Skip s [] s"
-| assignB: "big_step (var ::= e) s [] (upd s var (e s))"
-| basicB: "big_step (Basic f) s [] (upde s (f s))"
-| seqB: "big_step p1 s1 tr1 s2 \<Longrightarrow>
-         big_step p2 s2 tr2 s3 \<Longrightarrow>
-         big_step (p1; p2) s1 (tr1 @ tr2) s3"
-| condB1: "b s1 \<Longrightarrow> big_step p1 s1 tr s2 \<Longrightarrow> big_step (IF b THEN p1 ELSE p2 FI) s1 tr s2"
-| condB2: "\<not> b s1 \<Longrightarrow> big_step p2 s1 tr s2 \<Longrightarrow> big_step (IF b THEN p1 ELSE p2 FI) s1 tr s2"
-| waitB1: "e s > 0 \<Longrightarrow> big_step (Wait e) s [WaitBlk (e s) (\<lambda>_. s) ({}, {})] s"
-| waitB2: "\<not> e s > 0 \<Longrightarrow> big_step (Wait e) s [] s"
-| sendB1: "big_step (Cm (ch[!]e)) s [OutBlock ch (e s)] s"
-| sendB2: "(d::real) > 0 \<Longrightarrow> big_step (Cm (ch[!]e)) s
-            [WaitBlk d (\<lambda>_. s) ({ch}, {}), OutBlock ch (e s)] s"
-| receiveB1: "big_step (Cm (ch[?]var)) s [InBlock ch v] (upd s var v)"
-| receiveB2: "(d::real) > 0 \<Longrightarrow> big_step (Cm (ch[?]var)) s
-            [WaitBlk d (\<lambda>_. s) ({}, {ch}), InBlock ch v] (upd s var v)"
-| IChoiceB1: "big_step p1 s1 tr s2 \<Longrightarrow> big_step (IChoice p1 p2) s1 tr s2"
-| IChoiceB2: "big_step p2 s1 tr s2 \<Longrightarrow> big_step (IChoice p1 p2) s1 tr s2"
-| EChoiceSendB1: "i < length cs \<Longrightarrow> cs ! i = (Send ch e, p2) \<Longrightarrow>
-    big_step p2 s1 tr2 s2 \<Longrightarrow>
-    big_step (EChoice cs) s1 (OutBlock ch (e s1) # tr2) s2"
-| EChoiceSendB2: "(d::real) > 0 \<Longrightarrow> i < length cs \<Longrightarrow> cs ! i = (Send ch e, p2) \<Longrightarrow>
-    big_step p2 s1 tr2 s2 \<Longrightarrow>
-    big_step (EChoice cs) s1 (WaitBlk d (\<lambda>_. s1) (rdy_of_echoice cs) #
-                              OutBlock ch (e s1) # tr2) s2"
-| EChoiceReceiveB1: "i < length cs \<Longrightarrow> cs ! i = (Receive ch var, p2) \<Longrightarrow>
-    big_step p2 (upd s1 var v) tr2 s2 \<Longrightarrow>
-    big_step (EChoice cs) s1 (InBlock ch v # tr2) s2"
-| EChoiceReceiveB2: "(d::real) > 0 \<Longrightarrow> i < length cs \<Longrightarrow> cs ! i = (Receive ch var, p2) \<Longrightarrow>
-    big_step p2 (upd s1 var v) tr2 s2 \<Longrightarrow>
-    big_step (EChoice cs) s1 (WaitBlk d (\<lambda>_. s1) (rdy_of_echoice cs) #
-                              InBlock ch v # tr2) s2"
-| RepetitionB1: "big_step (Rep p) s [] s"
-| RepetitionB2: "big_step p s1 tr1 s2 \<Longrightarrow> big_step (Rep p) s2 tr2 s3 \<Longrightarrow>
-    tr = tr1 @ tr2 \<Longrightarrow>
-    big_step (Rep p) s1 tr s3"
-| ContB1: "\<not>b s \<Longrightarrow> big_step (Cont ode b) s [] s"
-| ContB2: "d > 0 \<Longrightarrow> ODEsol ode p d \<Longrightarrow>
-    (\<forall>t. t \<ge> 0 \<and> t < d \<longrightarrow> b (updr s1 (p t))) \<Longrightarrow>
-    \<not>b (updr s1 (p d)) \<Longrightarrow> p 0 = rpart s1 \<Longrightarrow>
-    big_step (Cont ode b) s1 [WaitBlk d (\<lambda>\<tau>. updr s1 (p \<tau>)) ({}, {})] (updr s1 (p d))"
-| InterruptSendB1: "i < length cs \<Longrightarrow> cs ! i = (Send ch e, p2) \<Longrightarrow>
-    big_step p2 s tr2 s2 \<Longrightarrow>
-    big_step (Interrupt ode b cs pr) s (OutBlock ch (e s) # tr2) s2"
-| InterruptSendB2: "d > 0 \<Longrightarrow> ODEsol ode p d \<Longrightarrow> p 0 = rpart s1 \<Longrightarrow>
-    (\<forall>t. t \<ge> 0 \<and> t < d \<longrightarrow> b (updr s1 (p t))) \<Longrightarrow>
-    i < length cs \<Longrightarrow> cs ! i = (Send ch e, p2) \<Longrightarrow>
-    rdy = rdy_of_echoice cs \<Longrightarrow>
-    big_step p2 (updr s1 (p d)) tr2 s2 \<Longrightarrow>
-    big_step (Interrupt ode b cs pr) s1 (WaitBlk d (\<lambda>\<tau>. updr s1 (p \<tau>)) rdy #
-                                         OutBlock ch (e (updr s1 (p d))) # tr2) s2"
-| InterruptReceiveB1: "i < length cs \<Longrightarrow> cs ! i = (Receive ch var, p2) \<Longrightarrow>
-    big_step p2 (upd s var v) tr2 s2 \<Longrightarrow>
-    big_step (Interrupt ode b cs pr) s (InBlock ch v # tr2) s2"
-| InterruptReceiveB2: "d > 0 \<Longrightarrow> ODEsol ode p d \<Longrightarrow> p 0 = rpart s1 \<Longrightarrow>
-    (\<forall>t. t \<ge> 0 \<and> t < d \<longrightarrow> b (updr s1 (p t))) \<Longrightarrow>
-    i < length cs \<Longrightarrow> cs ! i = (Receive ch var, p2) \<Longrightarrow>
-    rdy = rdy_of_echoice cs \<Longrightarrow>
-    big_step p2 (updr s1 ((p d)(var := v))) tr2 s2 \<Longrightarrow>
-    big_step (Interrupt ode b cs pr) s1 (WaitBlk d (\<lambda>\<tau>. updr s1 (p \<tau>)) rdy #
-                                         InBlock ch v # tr2) s2"
-| InterruptB1: "\<not>b s \<Longrightarrow> big_step pr s tr s2 \<Longrightarrow> big_step (Interrupt ode b cs pr) s tr s2"
-| InterruptB2: "d > 0 \<Longrightarrow> ODEsol ode p d \<Longrightarrow>
-    (\<forall>t. t \<ge> 0 \<and> t < d \<longrightarrow> b (updr s1 (p t))) \<Longrightarrow>
-    \<not>b (updr s1 (p d)) \<Longrightarrow> p 0 = rpart s1 \<Longrightarrow>
-    rdy = rdy_of_echoice cs \<Longrightarrow>
-    big_step pr (updr s1 (p d)) tr2 s2 \<Longrightarrow>
-    big_step (Interrupt ode b cs pr) s1 (WaitBlk d (\<lambda>\<tau>. updr s1 (p \<tau>)) rdy # tr2) s2"
-
-inductive_cases skipE: "big_step Skip s1 tr s2"
-inductive_cases assignE: "big_step (Assign var e) s1 tr s2"
-inductive_cases basicE: "big_step (Basic f) s1 tr s2"
-inductive_cases errorE: "big_step Error s1 tr s2"
-inductive_cases sendE: "big_step (Cm (ch[!]e)) s1 tr s2"
-inductive_cases receiveE: "big_step (Cm (ch[?]var)) s1 tr s2"
-inductive_cases seqE: "big_step (Seq p1 p2) s1 tr s2"
-inductive_cases condE: "big_step (Cond b p1 p2) s1 tr s2"
-inductive_cases waitE: "big_step (Wait d) s1 tr s2"
-inductive_cases echoiceE: "big_step (EChoice es) s1 tr s2"
-inductive_cases ichoiceE: "big_step (IChoice p1 p2) s1 tr s2"
-inductive_cases contE: "big_step (Cont ode b) s1 tr s2"
-inductive_cases interruptE: "big_step (Interrupt ode b cs pr) s1 tr s2"
-
-subsection \<open>Assertions on sequential processes\<close>
-
-text \<open>Assertion is a predicate on states and traces\<close>
-type_synonym 'a assn = "'a estate \<Rightarrow> 'a trace \<Rightarrow> bool"
-
-text \<open>We also define assertions parameterized by starting state\<close>
-type_synonym 'a assn2 = "'a estate \<Rightarrow> 'a assn"
-
-text \<open>Assertion stating the trace is empty\<close>
-definition emp :: "'a assn" where
-  "emp = (\<lambda>s tr. tr = [])"
-
-text \<open>True and false assertions\<close>
-inductive true_assn2 :: "'a assn2" where
-  "true_assn2 s0 s tr"
-
-definition false_assn2 :: "'a assn2" where
-  "false_assn2 = (\<lambda>s0 s tr. False)"
-
-text \<open>Quantifiers on assertions.\<close>
-definition forall_assn :: "('b \<Rightarrow> 'a assn) \<Rightarrow> 'a assn" (binder "\<forall>\<^sub>a" 10)where
-  "(\<forall>\<^sub>a n. P n) = (\<lambda>s tr. \<forall>n. P n s tr)"
-
-definition exists_assn :: "('b \<Rightarrow> 'a assn) \<Rightarrow> 'a assn" (binder "\<exists>\<^sub>a" 10)where
-  "(\<exists>\<^sub>a n. P n) = (\<lambda>s tr. \<exists>n. P n s tr)"
-
-text \<open>Substitution on assertions: real part.
-  Starting from a parameterized assertion P, let P act on the
-  state after making an assignment.
-\<close>
-definition subst_assn2 :: "'a assn2 \<Rightarrow> var \<Rightarrow> ('a estate \<Rightarrow> real) \<Rightarrow> 'a assn2"
-  ("_ {{_ := _}}" [90,90,90] 91) where 
-  "P {{var := e}} = (\<lambda>s0. P (upd s0 var (e s0)))"
-
-text \<open>Substitution on assertions: extra part.
-  Starting from a parameterized assertion P, let P act on the
-  state after updating the extra part using function f.  
-\<close>
-definition subste_assn2 :: "'a assn2 \<Rightarrow> ('a estate \<Rightarrow> 'a) \<Rightarrow> 'a assn2"
-  ("_ {{_}}" [90,90] 91) where 
-  "P {{f}} = (\<lambda>s0. P (upde s0 (f s0)))"
-
-definition disj_assn2 :: "'a assn2 \<Rightarrow> 'a assn2 \<Rightarrow> 'a assn2" (infixr "\<or>\<^sub>a" 35) where
-  "(P \<or>\<^sub>a Q) s0 = (\<lambda>s tr. P s0 s tr \<or> Q s0 s tr)"
-
-text \<open>Entailment relation between assertions\<close>
-definition entails :: "'a assn \<Rightarrow> 'a assn \<Rightarrow> bool" (infixr "\<Longrightarrow>\<^sub>A" 25) where
-  "(P \<Longrightarrow>\<^sub>A Q) \<longleftrightarrow> (\<forall>s tr. P s tr \<longrightarrow> Q s tr)"
-
-theorem entails_triv:
-  "P \<Longrightarrow>\<^sub>A P"
-  unfolding entails_def by auto
-
-lemma entails_trans:
-  "P \<Longrightarrow>\<^sub>A Q \<Longrightarrow> Q \<Longrightarrow>\<^sub>A R \<Longrightarrow> P \<Longrightarrow>\<^sub>A R"
-  unfolding entails_def by auto
-
-text \<open>Parameterized assertion specifying the initial condition
-  with starting state s0 and empty trace.
-\<close>
-definition init :: "'a assn2" where
-  "init s0 = (\<lambda>s tr. s = s0 \<and> tr = [])"
-
-text \<open>Conditional assertion\<close>
-definition cond_assn2 :: "'a eform \<Rightarrow> 'a assn2 \<Rightarrow> 'a assn2 \<Rightarrow> 'a assn2"
-  ("IFA _ THEN _ ELSE _ FI" [95,94] 93) where
-  "IFA b THEN Q1 ELSE Q2 FI = (\<lambda>s0 s tr. if b s0 then Q1 s0 s tr else Q2 s0 s tr)"
-
-text \<open>Assertion for input.
-
-  There are two cases, either the input happens immediately,
-  or after waiting for some time. The ensuing assertion is
-  parameterized by waiting time and communicated value.
-\<close>
-inductive wait_in_c :: "cname \<Rightarrow> (real \<Rightarrow> real \<Rightarrow> 'a assn2) \<Rightarrow> 'a assn2" where
-  "P 0 v s0 s tr \<Longrightarrow> wait_in_c ch P s0 s (InBlock ch v # tr)"
-| "0 < d \<Longrightarrow> P d v s0 s tr \<Longrightarrow> wait_in_c ch P s0 s (WaitBlk d (\<lambda>_. s0) ({}, {ch}) # InBlock ch v # tr)"
-
-text \<open>Assertion for output.
-
-  There are two cases, either the output happens immediately,
-  or after waiting for some time. The communicated value is
-  computed by the function e. The ensuing assertion is
-  parameterized by waiting time.
-\<close>
-inductive wait_out_c :: "cname \<Rightarrow> ('a estate \<Rightarrow> real) \<Rightarrow> (real \<Rightarrow> 'a assn2) \<Rightarrow> 'a assn2" where
-  "P 0 s0 s tr \<Longrightarrow> wait_out_c ch e P s0 s (OutBlock ch (e s0) # tr)"
-| "0 < d \<Longrightarrow> P d s0 s tr \<Longrightarrow> wait_out_c ch e P s0 s (WaitBlk d (\<lambda>_. s0) ({ch}, {}) # OutBlock ch (e s0) # tr)"
-
-text \<open>Waiting an amount of time, without state change\<close>
-inductive wait_c :: "'a eexp \<Rightarrow> 'a assn2 \<Rightarrow> 'a assn2" where
-  "e s0 > 0 \<Longrightarrow> P s0 s tr \<Longrightarrow> wait_c e P s0 s (WaitBlk (e s0) (\<lambda>_. s0) ({}, {}) # tr)"
-| "\<not>e s0 > 0 \<Longrightarrow> P s0 s tr \<Longrightarrow> wait_c e P s0 s tr"
-
-subsubsection \<open>Various rules about entailment\<close>
-
-lemma entails_exists:
-  assumes "\<exists>n. P \<Longrightarrow>\<^sub>A Q n"
-  shows "P \<Longrightarrow>\<^sub>A (\<exists>\<^sub>a n. Q n)"
-  using assms unfolding exists_assn_def entails_def
-  by auto
-
-lemma entails_assumption:
-  "P s \<Longrightarrow>\<^sub>A (IFA b THEN P ELSE true_assn2 FI) s"
-  unfolding cond_assn2_def entails_def
-  using true_assn2.intros by auto
-
-subsubsection \<open>Commutativity rules\<close>
-
-text \<open>The following rules state commutativity between
-  assertions and quantifiers.
-\<close>
-lemma wait_in_c_exists:
-  "wait_in_c ch (\<lambda>d v s0. \<exists>\<^sub>an. P d v s0 n) s0 = (\<exists>\<^sub>an. wait_in_c ch (\<lambda>d v s0. P d v s0 n) s0)"
-  apply (rule ext) apply (rule ext)
-  subgoal for s tr
-    apply (rule iffI)
-    subgoal unfolding exists_assn_def
-      apply (induct rule: wait_in_c.cases) apply auto
-      subgoal for v tr' n
-        apply (rule exI[where x=n])
-        apply (rule wait_in_c.intros(1)) by auto
-      subgoal for d v tr' n
-        apply (rule exI[where x=n])
-        apply (rule wait_in_c.intros(2)) by auto
-      done
-    subgoal unfolding exists_assn_def
-      apply auto subgoal for n
-        apply (induction rule: wait_in_c.cases) apply auto
-        subgoal for v tr'
-          apply (rule wait_in_c.intros(1))
-          apply (rule exI[where x=n]) by auto
-        subgoal for d v tr'
-          apply (rule wait_in_c.intros(2))
-           apply simp apply (rule exI[where x=n]) by auto
-        done
-      done
-    done
-  done
-
-lemma wait_out_c_exists:
-  "wait_out_c ch e (\<lambda>d s0. \<exists>\<^sub>a n. P d s0 n) s0 = (\<exists>\<^sub>a n. wait_out_c ch e (\<lambda>d s0. P d s0 n) s0)"
-  apply (rule ext) apply (rule ext)
-  subgoal for s tr
-    apply (rule iffI)
-    subgoal unfolding exists_assn_def
-      apply (induct rule: wait_out_c.cases) apply auto
-      subgoal for tr' n
-        apply (rule exI[where x=n])
-        apply (rule wait_out_c.intros(1)) by auto
-      subgoal for d tr' n
-        apply (rule exI[where x=n])
-        apply (rule wait_out_c.intros(2)) by auto
-      done
-    subgoal unfolding exists_assn_def
-      apply auto subgoal for n
-        apply (induction rule: wait_out_c.cases) apply auto
-        subgoal for tr'
-          apply (rule wait_out_c.intros(1))
-          apply (rule exI[where x=n]) by auto
-        subgoal for d tr'
-          apply (rule wait_out_c.intros(2))
-           apply simp apply (rule exI[where x=n]) by auto
-        done
-      done
-    done
-  done
-
-subsubsection \<open>Monotonicity rules\<close>
-
-text \<open>The following rules state monotonicity of assertions\<close>
-lemma wait_in_c_mono:
-  assumes "\<And>d v s. P1 d v s \<Longrightarrow>\<^sub>A P2 d v s"
-  shows "wait_in_c ch P1 s0 \<Longrightarrow>\<^sub>A wait_in_c ch P2 s0"
-  unfolding entails_def apply auto
-  subgoal for s tr
-    apply (induct rule: wait_in_c.cases) apply auto
-    subgoal for v tr'
-      apply (rule wait_in_c.intros(1))
-      using assms unfolding entails_def by auto
-    subgoal for d v tr'
-      apply (rule wait_in_c.intros(2))
-      using assms unfolding entails_def by auto
-    done
-  done
-
-lemma wait_out_c_mono:
-  assumes "\<And>d s. P1 d s \<Longrightarrow>\<^sub>A P2 d s"
-  shows "wait_out_c ch e P1 s0 \<Longrightarrow>\<^sub>A wait_out_c ch e P2 s0"
-  unfolding entails_def apply auto
-  subgoal for s tr
-    apply (induct rule: wait_out_c.cases) apply auto
-    subgoal for tr'
-      apply (rule wait_out_c.intros(1))
-      using assms unfolding entails_def by auto
-    subgoal for d tr'
-      apply (rule wait_out_c.intros(2))
-      using assms unfolding entails_def by auto
-    done
-  done
-
-subsection \<open>Hoare logic for sequential processes\<close>
-
-text \<open>Definition of Hoare triple\<close>
-definition Valid :: "'a assn \<Rightarrow> 'a proc \<Rightarrow> 'a assn \<Rightarrow> bool" ("\<Turnstile> ({(1_)}/ (_)/ {(1_)})" 50) where
-  "\<Turnstile> {P} c {Q} \<longleftrightarrow> (\<forall>s1 tr1 s2 tr2. P s1 tr1 \<longrightarrow> big_step c s1 tr2 s2 \<longrightarrow> Q s2 (tr1 @ tr2))"
-
-theorem strengthen_pre:
-  "\<Turnstile> {P2} c {Q} \<Longrightarrow> P1 \<Longrightarrow>\<^sub>A P2 \<Longrightarrow> \<Turnstile> {P1} c {Q}"
-  unfolding Valid_def entails_def by metis
-
-theorem weaken_post:
-  "\<Turnstile> {P} c {Q1} \<Longrightarrow> Q1 \<Longrightarrow>\<^sub>A Q2 \<Longrightarrow> \<Turnstile> {P} c {Q2}"
-  unfolding Valid_def entails_def by metis
-
-text \<open>Specification of a single process.
-
-  Each HCSP process can be specified using a parameterized
-  assertion, which for each starting state provides an assertion
-  on the ending state and trace.
-\<close>
-definition spec_of :: "'a proc \<Rightarrow> 'a assn2 \<Rightarrow> bool" where
-  "spec_of c Q \<longleftrightarrow> (\<forall>s0. \<Turnstile> {init s0} c {Q s0})"
-
-text \<open>Consequence rule for spec_of\<close>
-lemma spec_of_post:
-  "spec_of c Q1 \<Longrightarrow> \<forall>s0. Q1 s0 \<Longrightarrow>\<^sub>A Q2 s0 \<Longrightarrow> spec_of c Q2"
-  unfolding spec_of_def using weaken_post by blast
-
-subsubsection \<open>Hoare rules for basic commands\<close>
-
-text \<open>For each command, we state two versions of the rules,
-  one for the command alone, and one for the command followed
-  by an arbitrary process.
-\<close>
-
-text \<open>Hoare rule for skip statement\<close>
-lemma spec_of_skip:
-  "spec_of Skip init"
-  unfolding Valid_def spec_of_def
-  by (auto elim: skipE)
-
-lemma Valid_skip_sp:
-  assumes "spec_of c Q"
-  shows "spec_of (Skip; c) Q"
-  unfolding Valid_def spec_of_def
-  apply (auto elim!: seqE skipE)
-  using assms unfolding spec_of_def Valid_def init_def by auto
-
-text \<open>Hoare rule for assign\<close>
-lemma spec_of_assign:
-  "spec_of (var ::= e) (\<lambda>s0 s tr. s = upd s0 var (e s0))"
-  unfolding Valid_def spec_of_def init_def
-  by (auto elim!: assignE)
-
-lemma Valid_assign_sp:
-  assumes "spec_of c Q"
-  shows "spec_of (var ::= e; c) (Q {{ var := e }})"
-  unfolding Valid_def spec_of_def
-  apply (auto elim!: seqE assignE)
-  using assms unfolding spec_of_def Valid_def init_def subst_assn2_def by auto
-
-text \<open>Hoare rule for updating the extra state\<close>
-lemma spec_of_basic:
-  "spec_of (Basic f) (\<lambda>s0 s tr. s = upde s0 (f s0))"
-  unfolding Valid_def spec_of_def init_def
-  by (auto elim: basicE)
-
-lemma Valid_basic_sp:
-  assumes "spec_of c Q"
-  shows "spec_of (Basic f; c) (Q {{ f }})"
-  unfolding Valid_def spec_of_def
-  apply (auto elim!: seqE basicE)
-  using assms unfolding spec_of_def Valid_def init_def subste_assn2_def by auto
-
-lemma spec_of_ichoice:
-  assumes "spec_of c1 Q1"
-    and "spec_of c2 Q2"
-  shows "spec_of (IChoice c1 c2) (Q1 \<or>\<^sub>a Q2)"
-  unfolding Valid_def spec_of_def
-  apply (auto elim!: ichoiceE)
-  using assms unfolding spec_of_def Valid_def disj_assn2_def by auto
-
-text \<open>Hoare rule for error\<close>
-lemma spec_of_error:
-  "spec_of Error P"
-  unfolding Valid_def spec_of_def init_def
-  by (auto elim: errorE)
-
-lemma Valid_error_sp:
-  "spec_of (Error; c) Q"
-  unfolding Valid_def spec_of_def
-  by (auto elim: seqE errorE)
-
-text \<open>Hoare rules for conditional\<close>
-lemma spec_of_cond:
-  assumes "spec_of c1 Q1"
-    and "spec_of c2 Q2"
-  shows "spec_of (IF b THEN c1 ELSE c2 FI) (IFA b THEN Q1 ELSE Q2 FI)"
-  unfolding Valid_def spec_of_def init_def cond_assn2_def
-  apply (auto elim!: condE)
-  using assms unfolding Valid_def spec_of_def init_def by auto
-
-text \<open>Hoare rule for input\<close>
-lemma spec_of_receive:
-  "spec_of (Cm (ch[?]var)) (wait_in_c ch (\<lambda>d v. init {{ var := (\<lambda>_. v) }}))"
-  unfolding Valid_def spec_of_def init_def subst_assn2_def
-  apply (auto elim!: receiveE)
-   apply (rule wait_in_c.intros(1)) apply auto[1]
-  apply (rule wait_in_c.intros(2)) by auto
-
-lemma Valid_receive_sp:
-  assumes "spec_of c Q"
-  shows "spec_of (Cm (ch[?]var); c)
-                 (wait_in_c ch (\<lambda>d v. Q {{ var := (\<lambda>_. v) }}))"
-  using assms unfolding Valid_def spec_of_def init_def subst_assn2_def
-  apply (auto elim!: seqE receiveE)
-  apply (rule wait_in_c.intros(1)) apply auto[1]
-  using Valid_def spec_of_def init_def assms apply auto[1]
-  apply (rule wait_in_c.intros(2)) apply auto[1]
-  using Valid_def spec_of_def init_def assms apply auto[1]
-  done
-
-text \<open>Hoare rule for output\<close>
-lemma spec_of_send:
-  "spec_of (Cm (ch[!]e)) (wait_out_c ch e (\<lambda>d. init))"
-  unfolding Valid_def spec_of_def init_def
-  apply (auto elim!: sendE)
-   apply (rule wait_out_c.intros(1)) apply auto[1]
-  apply (rule wait_out_c.intros(2)) by auto
-
-lemma Valid_send_sp:
-  assumes "spec_of c Q"
-  shows "spec_of (Cm (ch[!]e); c)
-                 (wait_out_c ch e (\<lambda>d s0. Q s0))"
-  using assms unfolding Valid_def spec_of_def init_def
-  apply (auto elim!: seqE sendE)
-   apply (rule wait_out_c.intros(1))
-  using Valid_def spec_of_def init_def assms apply auto[1]
-  apply (rule wait_out_c.intros(2)) apply auto[1]
-  using Valid_def spec_of_def init_def assms apply auto[1]
-  done
-
-text \<open>Hoare rules for wait\<close>
-lemma spec_of_wait:
-  "spec_of (Wait e) (wait_c e init)"
-  unfolding Valid_def spec_of_def init_def
-  apply (auto elim!: waitE)
-   apply (rule wait_c.intros(1)) apply auto
-  apply (rule wait_c.intros(2)) by auto
-
-lemma Valid_wait_sp:
-  assumes "spec_of c Q"
-  shows "spec_of (Wait e; c) (wait_c e Q)"
-  using assms unfolding Valid_def spec_of_def init_def
-  apply (auto elim!: seqE waitE)
-   apply (rule wait_c.intros(1)) apply auto
-  apply (rule wait_c.intros(2)) by auto
-
-
-subsection \<open>Rewrite rules for big-step semantics\<close>
-
-text \<open>Repetition for n times\<close>
-fun RepN :: "nat \<Rightarrow> 'a proc \<Rightarrow> 'a proc" where
-  "RepN 0 c = Skip"
-| "RepN (Suc n) c = c; RepN n c"
-
-lemma big_step_rep:
-  "big_step (Rep c) s1 tr1 s2 \<longleftrightarrow> (\<exists>n. big_step (RepN n c) s1 tr1 s2)"
-proof -
-  have "big_step p s1 tr1 s2 \<Longrightarrow> p = Rep c \<Longrightarrow> \<exists>n. big_step (RepN n c) s1 tr1 s2" for p s1 tr1 s2
-    apply (induction rule: big_step.induct, auto)
-     apply (rule exI[where x=0])
-    apply simp apply (rule skipB)
-    subgoal for s1 tr1 s2 tr2 s3 n
-      apply (rule exI[where x="Suc n"])
-      apply simp apply (rule seqB) by auto
-    done
-  moreover have "\<And>s1 tr1 s2. big_step (RepN n c) s1 tr1 s2 \<Longrightarrow> big_step (Rep c) s1 tr1 s2" for n
-    apply (induction n)
-     apply simp apply (elim skipE) apply (auto intro: RepetitionB1)[1]
-    apply simp apply (elim seqE) apply (auto intro: RepetitionB2)
-    done
-  ultimately show ?thesis
-    by auto
-qed
-
-lemma spec_of_rep:
-  assumes "\<And>n. spec_of (RepN n c) (Q n)"
-  shows "spec_of (Rep c) (\<lambda>s0. \<exists>\<^sub>a n. Q n s0)"
-  using assms unfolding spec_of_def Valid_def big_step_rep exists_assn_def
-  by blast
-
-lemma big_step_seq_assoc:
-  "big_step ((p1; p2); p3) s1 tr s2 \<longleftrightarrow> big_step (p1; p2; p3) s1 tr s2"
-  apply (rule iffI)
-  subgoal apply (elim seqE)
-    apply auto apply (rule seqB) apply auto
-    apply (rule seqB) by auto
-  subgoal apply (elim seqE)
-    apply auto apply (subst append.assoc[symmetric])
-    apply (rule seqB) apply (rule seqB) by auto
-  done
-
-lemma spec_of_seq_assoc:
-  "spec_of ((p1; p2); p3) Q \<longleftrightarrow> spec_of (p1; p2; p3) Q"
-  unfolding spec_of_def Valid_def
-  using big_step_seq_assoc by blast
-
-lemma big_step_cond_distrib:
-  "big_step ((IF b THEN c1 ELSE c2 FI); c) s1 tr s2 \<longleftrightarrow>
-   big_step ((IF b THEN (c1; c) ELSE (c2; c) FI)) s1 tr s2"
-  apply (rule iffI)
-  subgoal apply (elim seqE)
-    subgoal for tr1 s3 tr2
-      apply (cases "b s1")
-      subgoal 
-        apply (rule condB1) apply simp
-        apply auto apply (rule seqB) by (auto elim: condE)
-      subgoal
-        apply (rule condB2) apply simp
-        apply auto apply (rule seqB) by (auto elim: condE)
-      done
-    done
-  subgoal apply (elim condE)
-    subgoal
-      apply (elim seqE) apply auto
-      apply (rule seqB) by (auto intro: condB1)
-    subgoal
-      apply (elim seqE) apply auto
-      apply (rule seqB) by (auto intro: condB2)
-    done
-  done
-
-lemma spec_of_cond_distrib:
-  "spec_of ((IF b THEN c1 ELSE c2 FI); c) Q \<longleftrightarrow>
-   spec_of ((IF b THEN (c1; c) ELSE (c2; c) FI)) Q"
-  unfolding spec_of_def Valid_def
-  using big_step_cond_distrib by blast
 
 subsection \<open>States for parallel programs\<close>
 
@@ -734,6 +12,9 @@ text \<open>Merge of two states.
 \<close>
 definition merge_state :: "'a gstate \<Rightarrow> 'a gstate \<Rightarrow> 'a gstate" where
   "merge_state ps1 ps2 = (\<lambda>p. case ps1 p of None \<Rightarrow> ps2 p | Some s \<Rightarrow> Some s)"
+
+definition restrict_state :: "pname set \<Rightarrow> 'a gstate \<Rightarrow> 'a gstate" where
+  "restrict_state pns gs = (\<lambda>pn. if pn \<in> pns then gs pn else None)"
 
 text \<open>Set of processes in a parallel state.\<close>
 definition proc_set :: "'a gstate \<Rightarrow> pname set" where
@@ -748,6 +29,11 @@ lemma proc_set_merge [simp]:
   apply (auto simp add: proc_set_def merge_state_def)
   subgoal for x y apply (cases "s1 x") by auto
   done
+
+lemma proc_set_restrict_state:
+  assumes "pns1 \<subseteq> proc_set s"
+  shows "proc_set (restrict_state pns1 s) = pns1"
+  using assms unfolding restrict_state_def proc_set_def by auto
 
 text \<open>Updating the global state: real part\<close>
 definition updg :: "'a gstate \<Rightarrow> pname \<Rightarrow> var \<Rightarrow> real \<Rightarrow> 'a gstate" where
@@ -843,6 +129,50 @@ lemma merge_state_eval2:
   using assms apply (auto simp add: merge_state_def proc_set_def)
   apply (cases "s11 pn") by auto
 
+lemma restrict_state_eval1:
+  assumes "proc_set gs1 = pns1"
+  shows "restrict_state pns1 (merge_state gs1 gs2) = gs1"
+  apply (rule ext) subgoal for pn
+    unfolding restrict_state_def apply auto
+     apply (subst merge_state_eval1) using assms apply auto
+    unfolding proc_set_def by auto
+  done
+
+lemma restrict_state_eval2:
+  assumes "proc_set gs1 = pns1"
+    and "proc_set gs2 = pns2"
+    and "pns1 \<inter> pns2 = {}"
+  shows "restrict_state pns2 (merge_state gs1 gs2) = gs2"
+  apply (rule ext) subgoal for pn
+    unfolding restrict_state_def apply auto
+     apply (subst merge_state_eval2) using assms apply auto
+    unfolding proc_set_def by auto
+  done
+
+lemma merge_restrict:
+  assumes "proc_set s = pns1 \<union> pns2"
+    and "pns1 \<inter> pns2 = {}"
+  shows "merge_state (restrict_state pns1 s) (restrict_state pns2 s) = s"
+  unfolding merge_state_def restrict_state_def
+  apply (rule ext) apply auto
+  using assms(1,2) unfolding proc_set_def apply auto
+  subgoal for p apply (cases "s p") by auto
+  subgoal for p apply (cases "s p") by auto
+  done
+
+lemma merge_state_elim:
+  assumes "proc_set s = pns1 \<union> pns2"
+    and "pns1 \<inter> pns2 = {}"
+    and "\<And>s1 s2. s = merge_state s1 s2 \<Longrightarrow> proc_set s1 = pns1 \<Longrightarrow> proc_set s2 = pns2 \<Longrightarrow> P"
+  shows P
+  apply (rule assms(3)[of "restrict_state pns1 s" "restrict_state pns2 s"])
+  by (auto simp add: merge_restrict proc_set_restrict_state assms)  
+
+lemma valg_merge_state_left:
+  assumes "pn \<in> proc_set s1"
+  shows "valg (merge_state s1 s2) pn v = valg s1 pn v"
+  using assms by (auto simp add: proc_set_def merge_state_def valg_def)
+
 lemma single_subst_merge_state1:
   assumes "pn \<in> proc_set s11"
   shows "updg (merge_state s11 s12) pn var e = merge_state (updg s11 pn var e) s12"
@@ -888,6 +218,10 @@ subsection \<open>Semantics of parallel processes\<close>
 text \<open>Whether two ready info from different processes are compatible\<close>
 fun compat_rdy :: "rdy_info \<Rightarrow> rdy_info \<Rightarrow> bool" where
   "compat_rdy (r11, r12) (r21, r22) = (r11 \<inter> r22 = {} \<and> r12 \<inter> r21 = {})"
+
+lemma compat_rdy_empty [simp]:
+  "compat_rdy rdy ({}, {})"
+  apply (cases rdy) by auto
 
 text \<open>Merge two ready info, common channels are removed\<close>
 fun merge_rdy :: "cname set \<Rightarrow> rdy_info \<Rightarrow> rdy_info \<Rightarrow> rdy_info" where
@@ -1615,6 +949,38 @@ lemma pure_gassn_intro:
   shows "P \<Longrightarrow>\<^sub>g !\<^sub>g[b]"
   using assms unfolding pure_gassn_def entails_g_def by auto
 
+lemma exists_gassn_elim:
+  assumes "\<And>n. P n \<Longrightarrow>\<^sub>g Q"
+  shows "(\<exists>\<^sub>g n. P n) \<Longrightarrow>\<^sub>g Q"
+  using assms unfolding exists_gassn_def entails_g_def
+  by auto
+
+lemma conj_pure_gassn_elim:
+  assumes "R \<Longrightarrow> P \<Longrightarrow>\<^sub>g Q"
+  shows "(!\<^sub>g[R] \<and>\<^sub>g P) \<Longrightarrow>\<^sub>g Q"
+  using assms unfolding entails_g_def conj_gassn_def pure_gassn_def
+  by auto
+
+lemma entails_g_disj:
+  assumes "P1 gs0 \<Longrightarrow>\<^sub>g R gs0"
+    and "P2 gs0 \<Longrightarrow>\<^sub>g R gs0"
+  shows "(P1 \<or>\<^sub>g P2) gs0 \<Longrightarrow>\<^sub>g R gs0"
+  using assms unfolding entails_g_def disj_gassn_def by auto
+
+lemma entails_g_disj2:
+  assumes "P1 gs0 \<Longrightarrow>\<^sub>g R1 gs0"
+    and "P2 gs0 \<Longrightarrow>\<^sub>g R2 gs0"
+  shows "(P1 \<or>\<^sub>g P2) gs0 \<Longrightarrow>\<^sub>g (R1 \<or>\<^sub>g R2) gs0"
+  using assms unfolding entails_g_def disj_gassn_def by auto
+
+lemma cond_gassn_true:
+  "b \<Longrightarrow> (IFG [pn] (\<lambda>_. b) THEN P ELSE Q FI = P)"
+  unfolding cond_gassn2_def by auto
+
+lemma cond_gassn_false:
+  "\<not>b \<Longrightarrow> (IFG [pn] (\<lambda>_. b) THEN P ELSE Q FI = Q)"
+  unfolding cond_gassn2_def by auto
+
 lemma sync_gassn_false_left:
   "sync_gassn chs pns1 pns2 false_gassn Q s0 \<Longrightarrow>\<^sub>g R s0"
   unfolding entails_g_def apply auto
@@ -1652,30 +1018,6 @@ lemma sync_gassn_disj2:
     using assms unfolding disj_gassn_def entails_g_def
     by (auto simp add: sync_gassn.intros)
   done
-
-lemma exists_gassn_elim:
-  assumes "\<And>n. P n \<Longrightarrow>\<^sub>g Q"
-  shows "(\<exists>\<^sub>g n. P n) \<Longrightarrow>\<^sub>g Q"
-  using assms unfolding exists_gassn_def entails_g_def
-  by auto
-
-lemma conj_pure_gassn_elim:
-  assumes "R \<Longrightarrow> P \<Longrightarrow>\<^sub>g Q"
-  shows "(!\<^sub>g[R] \<and>\<^sub>g P) \<Longrightarrow>\<^sub>g Q"
-  using assms unfolding entails_g_def conj_gassn_def pure_gassn_def
-  by auto
-
-lemma entails_g_disj:
-  assumes "P1 gs0 \<Longrightarrow>\<^sub>g R gs0"
-    and "P2 gs0 \<Longrightarrow>\<^sub>g R gs0"
-  shows "(P1 \<or>\<^sub>g P2) gs0 \<Longrightarrow>\<^sub>g R gs0"
-  using assms unfolding entails_g_def disj_gassn_def by auto
-
-lemma entails_g_disj2:
-  assumes "P1 gs0 \<Longrightarrow>\<^sub>g R1 gs0"
-    and "P2 gs0 \<Longrightarrow>\<^sub>g R2 gs0"
-  shows "(P1 \<or>\<^sub>g P2) gs0 \<Longrightarrow>\<^sub>g (R1 \<or>\<^sub>g R2) gs0"
-  using assms unfolding entails_g_def disj_gassn_def by auto
 
 lemma sync_gassn_ifg_left:
   assumes
@@ -1722,14 +1064,6 @@ lemma sync_gassn_ifg_left:
     qed
     done
   done
-
-lemma cond_gassn_true:
-  "b \<Longrightarrow> (IFG [pn] (\<lambda>_. b) THEN P ELSE Q FI = P)"
-  unfolding cond_gassn2_def by auto
-
-lemma cond_gassn_false:
-  "\<not>b \<Longrightarrow> (IFG [pn] (\<lambda>_. b) THEN P ELSE Q FI = Q)"
-  unfolding cond_gassn2_def by auto
 
 lemma sync_gassn_true_left:
   assumes "proc_set_gassn pns2 Q"
@@ -1874,6 +1208,16 @@ lemma sync_gassn_exists_right:
   done
 
 subsubsection \<open>Monotonicity rules\<close>
+
+lemma exists_gassn_mono:
+  assumes "\<And>n. P1 n \<Longrightarrow>\<^sub>g P2 n"
+  shows "(\<exists>\<^sub>gn. P1 n) \<Longrightarrow>\<^sub>g (\<exists>\<^sub>gn. P2 n)"
+  using assms unfolding entails_g_def exists_gassn_def by auto
+
+lemma conj_pure_gassn_mono:
+  assumes "b \<Longrightarrow> Q1 \<Longrightarrow>\<^sub>g Q2"
+  shows "(!\<^sub>g[b] \<and>\<^sub>g Q1) \<Longrightarrow>\<^sub>g (!\<^sub>g[b] \<and>\<^sub>g Q2)"
+  using assms unfolding entails_g_def conj_gassn_def pure_gassn_def by auto
 
 lemma cond_gassn_mono:
   assumes "P1 s0 \<Longrightarrow>\<^sub>g P2 s0"
